x86/RelocBingenproof.v
@@ -1,0 +1,97 @@
+(* *******************  *)
+(* Author: Jinhua Wu    *)
+(* Date:   Jul 26th     *)
+(* *******************  *)
+
+Require Import Coqlib Maps AST lib.Integers Values.
+Require Import Events lib.Floats Memory Smallstep.
+Require Import Asm RelocProg RelocProgram Globalenvs.
+Require Import Stacklayout Conventions.
+Require Import Linking Errors.
+Require Import EncDecRet RelocBingen RelocBinDecode.
+Require Import TranslateInstr RelocProgSemantics2.
+
+Import ListNotations.
+Local Open Scope error_monad_scope.
+  
+Section WITH_INSTR_SIZE.
+
+Variable instr_size : instruction -> Z.
+Variable Instr_size : list Instruction -> Z.
+
+Hypothesis translate_instr_size: forall i e l l',
+      translate_instr e i = OK l ->
+      Instr_size (l ++ l') = instr_size i.
+
+Definition match_prog (p: program) (tp: program) :=
+  transf_program instr_size p = OK tp.
+
+Lemma decode_prog_code_section_total: forall p tp,
+    transf_program instr_size p = OK tp ->
+    exists tp', decode_prog_code_section instr_size Instr_size tp = OK tp'.
+Proof.
+Admitted.
+
+
+
+Section PRESERVATION. 
+(** Transformation *)
+Variable prog: program.
+Variable tprog: program.
+Hypothesis TRANSF: match_prog prog tprog.
+
+Let ge := RelocProgSemantics.globalenv instr_size prog.
+Let tge := globalenv instr_size Instr_size tprog.
+
+
+
+Definition match_instr (i1 i2: instruction):=
+  forall e l l', translate_instr e i1 = OK l ->
+         decode_instr e (l ++ l') = OK (i2,l').
+
+
+(* instruction map is mostly identical *)
+Lemma find_instr_refl: forall b ofs i,
+    RelocProgSemantics.Genv.genv_instrs ge b ofs = Some i ->
+    exists i1, RelocProgSemantics.Genv.genv_instrs tge b ofs = Some i
+          /\ match_instr i i1.
+Proof.
+  unfold ge,tge. unfold globalenv.
+  unfold match_prog in TRANSF.
+  exploit decode_prog_code_section_total;eauto.
+  intros (tp' & A). rewrite A.
+  simpl.
+  unfold transf_program in *. monadInv TRANSF.
+  unfold transl_sectable in EQ.
+  unfold decode_prog_code_section in *.
+  monadInv A. simpl in *.
+  clear ge tge.
+Admitted.
+
+
+Lemma transf_initial_state:forall st1 rs,
+    RelocProgSemantics1.initial_state instr_size prog rs st1 ->
+    exists st2, initial_state instr_size Instr_size tprog rs st2 /\ st1 = st2.
+  intros st1 rs H.
+  inv H. inv H1.
+  unfold match_prog in TRANSF.
+  exploit decode_prog_code_section_total;eauto.
+  intros (tp' & A).
+  
+  assert (TOPROVE: init_mem instr_size tp' = Some m).
+  { unfold RelocProgSemantics.init_mem in H.
+    unfold init_mem.
+    simpl in H. destr_in H.
+    assert (alloc_sections (RelocProgSemantics.globalenv instr_size tp')
+      (prog_symbtable tp') (prog_reloctables tp') 
+      (prog_sectable tp') Mem.empty = Some m0).
+    (* ge relation *)
+    unfold decode_prog_code_section in A.
+    monadInv A. simpl.
+    unfold transf_program in TRANSF. monadInv TRANSF.
+    unfold transl_sectable in  EQ0. simpl in *.
+    exploit PTree_fold_elements. apply EQ. intros F1. clear EQ.
+    exploit PTree_fold_elements. apply EQ0. intros F2. clear EQ0.
+    
+Admitted.
+
